proof-libs/fstar/rust_primitives/Rust_primitives.Hax.Folds.fsti
@@ -50,7 +50,7 @@ val fold_enumerated_slice
   : result: acc_t {inv result (length s)}
 
 (**** `(start..end_).step_by(step)` *)
-unfold let fold_range_step_by_wf_index (#u: Lib.IntTypes.inttype)
+unfold let fold_range_step_by_wf_index (#u: inttype)
   (start: int_t u) (end_: int_t u)
   (step: usize {v step > 0}) (strict: bool) (i: int)
   = v start < v end_ ==> (let end_step = v end_ - 1 - ((v end_ - 1 - v start) % v step) in
@@ -59,7 +59,7 @@ unfold let fold_range_step_by_wf_index (#u: Lib.IntTypes.inttype)
   // /\ i % v step == v start % v step
 
 #push-options "--z3rlimit 80"
-unfold let fold_range_step_by_upper_bound (#u: Lib.IntTypes.inttype)
+unfold let fold_range_step_by_upper_bound (#u: inttype)
   (start: int_t u) (end_: int_t u)
   (step: usize {v step > 0})
   : end':int {fold_range_step_by_wf_index start end_ step false end'}
@@ -76,7 +76,7 @@ unfold let fold_range_step_by_upper_bound (#u: Lib.IntTypes.inttype)
 /// Fold function that is generated for `for` loops iterating on
 /// `s.enumerate()`-like iterators
 val fold_range_step_by
-  (#acc_t: Type0) (#u: Lib.IntTypes.inttype)
+  (#acc_t: Type0) (#u: inttype)
   (start: int_t u)
   (end_: int_t u)
   (step: usize {v step > 0 /\ range (v end_ + v step) u})
@@ -87,7 +87,7 @@ val fold_range_step_by
   : result: acc_t {inv result (mk_int (fold_range_step_by_upper_bound start end_ step))}
 
 (**** `start..end_` *)
-unfold let fold_range_wf_index (#u: Lib.IntTypes.inttype)
+unfold let fold_range_wf_index (#u: inttype)
   (start: int_t u) (end_: int_t u)
   (strict: bool) (i: int)
   = v start <= v end_
@@ -95,7 +95,7 @@ unfold let fold_range_wf_index (#u: Lib.IntTypes.inttype)
      /\ (if strict then i < v end_ else i <= v end_))
 
 let rec fold_range
-  (#acc_t: Type0) (#u: Lib.IntTypes.inttype)
+  (#acc_t: Type0) (#u: inttype)
   (start: int_t u)
   (end_: int_t u)
   (inv: acc_t -> (i:int_t u{fold_range_wf_index start end_ false (v i)}) -> Type0)
