proof-libs/fstar/core/Core.Num.fsti
@@ -102,3 +102,5 @@ unfold instance sub_assign_num t
     f_sub_assign_post = (fun x y r -> x -. y = r);
     f_sub_assign = (fun x y -> x -. y);
   }
+
+
